fix soundness.v after "Don't carry around value types in the ast types."

src/ast.v
@@ -54,9 +54,9 @@ Function type_of_value (v: value): type :=
    | v_nat _ => t_nat
    | v_bool _ => t_bool
    | v_pair a b => t_pair (type_of_value a) (type_of_value b)
-   | v_list t l => t
-   | v_addr (mkaddr ty _ _) => ty
-   | v_lock (mkaddr ty _ _) => ty
+   | v_list t l => t_list t
+   | v_addr (mkaddr ty _ _) => t_addr ty
+   | v_lock (mkaddr ty _ _) => t_lock ty
    | v_undef => t_unit (* XXX *)
    end.
 
